Vizing/Aux.lean
@@ -1,3 +1,4 @@
 import Vizing.Aux.SetSet
 import Vizing.Aux.TakeUntil
 import Vizing.Aux.Upstream
+import Vizing.Aux.Adjacent
