Vizing/InversionGuarantee.lean
@@ -8,19 +8,99 @@ open Aux Graph EdgeColoring Fan Path
 
 variable
   {n c : Nat} {G : Graph n} (C : EdgeColoring c G)
-  {x y : Vertex n} {a b : Color c} (ha : a.isSome)
+  {x y : Vertex n} {a b : Color c} (ha : a.isSome) (hb : b.isSome)
 
 -- Maximality : all free colors on last vertex of fan are free on x
 
+include ha hb in
+theorem freeColors_inversion_invariant {C' : EdgeColoring c G} {P : Path C a b x}
+  {u : Vertex n} {d : Color c}
+  (hC' : isInverted C C' P) (hu : u ≠ P.val.head (P.nonemptyAx) ∧ u ≠ P.val.getLast (P.nonemptyAx))
+  (hd : d ∈ freeColorsOn C u) : d ∈ freeColorsOn C' u := by
+  have : d.isSome :=
+    by exact isSome_if_mem_freeColorsOn C u hd
+  apply freeColor_of_not_exists_and_isSome
+  · assumption
+  · apply not_exists_of_freeColor at hd
+    contrapose! hd
+    rcases hd with ⟨v, hv⟩
+    rcases hC' with ⟨hnotmem, hmem⟩
+    by_cases h : (u, v) ∈ pathEdges P
+    · specialize hmem (u, v) h
+      rcases exists_other_nbor_of_mem_pathEdges ha hb h hu with ⟨w, hw1, hw2⟩
+      use w
+      apply color_of_mem_pathEdges at h
+      apply color_of_mem_pathEdges at hw1
+      simp_all
+      grind
+    · specialize hnotmem (u, v)
+      use v
+      rwa [hnotmem]
+      rw [← mem_edgeSet_iff_present]
+      apply C'.representsEdgesAx
+      rwa [← color.eq_def, hv]
+      assumption
+
+
+theorem colorAx_invariant
+  {C' : EdgeColoring c G} {F : List (Vertex n)} (hF : F ≠ [])
+  (hF2 : F.Nodup)
+  (h1 : ∀ (a b : Vertex n), (a, b) ∈ (toEdgeSet G).val → color C (a, b) = color C' (a, b))
+  (h2 : List.Chain' (fun f₁ f₂ ↦ color C (x, f₂) ∈ freeColorsOn C f₁) F)
+  (h3 : ∀ z ∈ F, z ≠ F.head hF → (color C (x, z)).isSome) :
+  List.Chain' (fun f₁ f₂ ↦ color C' (x, f₂) ∈ freeColorsOn C' f₁) F := by
+  induction' F
+  · trivial
+  · rename_i head tail ih
+    apply List.Chain'.cons'
+    by_cases htail : tail = []
+    · subst htail
+      trivial
+    apply ih
+    · exact List.Nodup.of_cons hF2
+    · apply List.Chain'.tail at h2
+      simpa using h2
+    · intro z hz1 hz2
+      have := List.mem_cons_of_mem head hz1
+      apply h3
+      · exact this
+      · simp only [List.head_cons]
+        by_contra hc
+        rw [hc] at hz1
+        exact List.Nodup.notMem hF2 hz1
+    · assumption
+    · intro z hz
+      have aux : (x, z) ∈ (toEdgeSet G).val := by
+        rw [← mem_edgeSet_iff_present]
+        apply C.representsEdgesAx
+        apply h3
+        · exact List.mem_cons_of_mem head (List.mem_of_mem_head? hz)
+        · grind
+      rcases List.chain'_cons'.mp h2 with ⟨h4, _⟩
+      specialize h4 z hz
+      have : ∀ a, a ∈ freeColorsOn C head → a ∈ freeColorsOn C' head := by
+        intro a ha
+        have h5 : a.isSome := by exact isSome_if_mem_freeColorsOn C head ha
+        apply freeColor_of_not_exists_and_isSome
+        · assumption
+        apply not_exists_of_freeColor at ha
+        contrapose! ha
+        rcases ha with ⟨v, hv⟩
+        use v
+        rwa [h1]
+        · rw [← mem_edgeSet_iff_present]
+          apply C'.representsEdgesAx
+          rwa [← color.eq_def, hv]
+      rw [← h1]
+      tauto
+      assumption
+
 include ha in
 theorem inversion_guarantee (F : Fan C x y)
-  {C' : EdgeColoring c G}
-  {P : Path C a b x}
-  (hC' : isInverted C C' P)
-  (ha1 : a ∈ freeColorsOn C (last F))
-  (hF : isMaximal F)
-  (hxy : color C (x, y) = none) :
-  ∃ i : Fin F.val.size, a ∈ freeColorsOn C' F.val[i] := by
+  {C' : EdgeColoring c G} {P : Path C a b x}
+  (hC' : isInverted C C' P) (ha1 : a ∈ freeColorsOn C (last F))
+  (hF : isMaximal F) (hxy : color C (x, y) = none) :
+  ∃ i : Fin F.val.size, a ∈ freeColorsOn C' F.val[i] ∧ colorAx C' (Array.extract F.val 0 (i+1)) x := by
   by_cases h : ∃ j : Fin F.val.size, color C (x, F.val[j]) = a
   rcases h with ⟨j, hj⟩
   have aux0 : j.val > 0 := by
@@ -34,51 +114,56 @@ theorem inversion_guarantee (F : Fan C x y)
     omega
   by_cases hp : F.val[j.val - 1] ∈ P.val
   · use ⟨F.val.size - 1, (by simp; apply Array.size_pos_iff.mpr; exact F.nonemptyAx)⟩
-    apply freeColor_of_not_exists_and_isSome _ ha
-    simp [isInverted, isInverted_notmem, isInverted_mem, aux1, pathEdges, color] at hC'
-    rcases hC' with ⟨hC', _⟩
-    have ha2 := not_exists_of_freeColor C ha1
-    contrapose! ha2
-    rcases ha2 with ⟨v, hv⟩
-    use v
-    rw [← hv]
-    simp [color, last, Array.back_eq_getElem]
-    apply hC'
-    · rw [← mem_edgeSet_iff_present]
-      apply C'.representsEdgesAx
-      simp [color] at ⊢ hv
-      rwa [hv]
-    · by_contra hc
-      simp [last, Array.back] at ha1
-      simp [isMaximal] at hF
-      apply mem_pathEdges_if at hc
-      simp at hc
-      have : F.val[F.val.size - 1] ≠ F.val[j.val - 1] := by
-        by_contra hc
-        apply (List.Nodup.getElem_inj_iff F.nodupAx).mp at hc
-        have : j = F.val.size := by omega
-        have := j.isLt
-        omega
-      have := isLast_if C hp aux1
-      have := isLast_if C hc.left ha1
-      simp_all
+    constructor
+    · apply freeColor_of_not_exists_and_isSome _ ha
+      simp [isInverted, isInverted_notmem, isInverted_mem, aux1, pathEdges, color] at hC'
+      rcases hC' with ⟨hC', _⟩
+      have ha2 := not_exists_of_freeColor C ha1
+      contrapose! ha2
+      rcases ha2 with ⟨v, hv⟩
+      use v
+      rw [← hv]
+      simp [color, last, Array.back_eq_getElem]
+      apply hC'
+      · rw [← mem_edgeSet_iff_present]
+        apply C'.representsEdgesAx
+        simp [color] at ⊢ hv
+        rwa [hv]
+      · by_contra hc
+        simp [last, Array.back] at ha1
+        simp [isMaximal] at hF
+        apply mem_pathEdges_if at hc
+        simp at hc
+        have : F.val[F.val.size - 1] ≠ F.val[j.val - 1] := by
+          by_contra hc
+          apply (List.Nodup.getElem_inj_iff F.nodupAx).mp at hc
+          have : j = F.val.size := by omega
+          have := j.isLt
+          omega
+        have := isLast_if C hp aux1
+        have := isLast_if C hc.left ha1
+        simp_all
+    ·
+      sorry
   · use ⟨j.val - 1, Nat.sub_lt_of_lt j.isLt⟩
-    apply freeColor_of_not_exists_and_isSome _ ha
-    apply not_exists_of_freeColor at aux1
-    contrapose! aux1
-    rcases aux1 with ⟨v, hv⟩
-    use v
-    rw [← hv]
-    simp [isInverted, isInverted_notmem] at hC'
-    rcases hC' with ⟨hC', _⟩
-    apply hC'
-    · rw [← mem_edgeSet_iff_present]
-      apply C'.representsEdgesAx
-      simp [color] at ⊢ hv
-      rwa [hv]
-    · apply not_mem_pathEdges_if
-      left
-      trivial
+    constructor
+    · apply freeColor_of_not_exists_and_isSome _ ha
+      apply not_exists_of_freeColor at aux1
+      contrapose! aux1
+      rcases aux1 with ⟨v, hv⟩
+      use v
+      rw [← hv]
+      simp [isInverted, isInverted_notmem] at hC'
+      rcases hC' with ⟨hC', _⟩
+      apply hC'
+      · rw [← mem_edgeSet_iff_present]
+        apply C'.representsEdgesAx
+        simp [color] at ⊢ hv
+        rwa [hv]
+      · apply not_mem_pathEdges_if
+        left
+        trivial
+    · sorry
   have aux0 : a ∈ freeColorsOn C x := by
     simp [isMaximal] at hF
     by_contra hc
@@ -118,19 +203,50 @@ theorem inversion_guarantee (F : Fan C x y)
         simp_all [color]
       simp_all [color, freeColorsOn, incidentColorsOn, Option.isSome_iff_ne_none]
   use ⟨F.val.size - 1, (by simp; apply Array.size_pos_iff.mpr; exact F.nonemptyAx)⟩
-  apply freeColor_of_not_exists_and_isSome _ ha
   simp [isInverted, isInverted_notmem, isInverted_mem, aux1, pathEdges, color] at hC'
-  apply not_exists_of_freeColor at ha1
-  contrapose! ha1
-  rcases ha1 with ⟨v, hv⟩
-  use v
-  rw [← hv]
-  simp [color, last, Array.back_eq_getElem]
-  apply hC'
-  rw [← mem_edgeSet_iff_present]
-  apply C'.representsEdgesAx
-  simp [color] at ⊢ hv
-  rwa [hv]
+  constructor
+  · apply freeColor_of_not_exists_and_isSome _ ha
+    apply not_exists_of_freeColor at ha1
+    contrapose! ha1
+    rcases ha1 with ⟨v, hv⟩
+    use v
+    rw [← hv]
+    simp [color, last, Array.back_eq_getElem]
+    apply hC'
+    rw [← mem_edgeSet_iff_present]
+    apply C'.representsEdgesAx
+    simp [color] at ⊢ hv
+    rwa [hv]
+  · have hcolor := F.colorAx
+    have : (F.val.size - 1 + 1) = F.val.size := by
+      apply Nat.sub_add_cancel
+      apply Nat.succ_le_of_lt
+      exact Array.size_pos_iff.mpr F.nonemptyAx
+    simp [this]
+    unfold colorAx fan_prop color at ⊢ hcolor
+    -- simp at ⊢ hcolor
+    simp_all
+    induction' F.val.toList
+    · trivial
+    · rename_i head tail ih
+      apply List.Chain'.cons' ih
+      intro z hz
+      rw [← hC']
+      · sorry
+      · rw [← mem_edgeSet_iff_present]
+        apply C.representsEdgesAx
+        simp
+        apply fan_colored_edges x y F
+        stop
+
+
+
+
+    -- Lemma : inverted path : freeColorsOn remain the same for everything except first and last ..?
+
+
+
+        sorry
 
 def findSubfanWithColor (F : Fan C x y)
   (C' : EdgeColoring c G)
@@ -153,6 +269,7 @@ def findSubfanWithColor (F : Fan C x y)
     simp [colorAx]
     apply List.Chain'.prefix (l := F.val.toList)
     · unfold fan_prop
+
       -- Path inversion guarantee
       sorry
     · simp [← List.isPrefixOf_iff_prefix, Array.isPrefixOf_toList]
